unfold pred_n

ThoR/Semantics/Semantics.lean
@@ -23,7 +23,7 @@ inductive TyTy : Type 1 where
     | formula : Ty .isTy -- Prop
     | expression : {n : ℕ} → (rel_type : RelType R n) → Ty .isTy-- Rel rel_type
     | function : {n : ℕ} → (t : RelType R n) → Ty .isTy → Ty .isTy -- type1.eval → type2.eval
-    | pred : {n : ℕ} → {t : RelType R n} → Ty (.isPred t) → Ty .isTy
+--    | pred : {n : ℕ} → {t : RelType R n} → Ty (.isPred t) → Ty .isTy
     | pred_1 : {n : ℕ} → (t : RelType R n) → Ty (.isPred t)
     | pred_n : {n : ℕ} → (t : RelType R n) → Ty (.isPred t) → Ty (.isPred t)
 
@@ -38,7 +38,7 @@ inductive TyTy : Type 1 where
     | .formula => Prop
     | .expression rel_type => Rel rel_type
     | .function dom_rel_type ran => Rel dom_rel_type → ran.eval
-    | .pred p => p.eval
+  --  | .pred p => p.eval
     | .pred_1 dom_rel_type => Rel dom_rel_type → Prop
     | .pred_n dom_rel_type p' => Rel dom_rel_type → (p'.eval)
 
@@ -57,223 +57,223 @@ inductive TyTy : Type 1 where
     | global_rel_var {n : ℕ} {t : RelType R n} (r : Rel t) (name : String): Term (.expression t)
     | local_rel_var {n : ℕ} {t : RelType R n} (r : Rel t): Term (.expression t)
 
-    /- expression constants -/
-    --| univ
-    --| none
-    --| iden
+    -- /- expression constants -/
+    -- --| univ
+    -- --| none
+    -- --| iden
 
-    /- binary expression operators -/
-    | union
-      {n : ℕ}
-      {t1 t2 : RelType R n}
-      : Term (.expression t1) →
-        Term (.expression t2) →
-        Term (.expression (t1 + t2))
+    -- /- binary expression operators -/
+    -- | union
+    --   {n : ℕ}
+    --   {t1 t2 : RelType R n}
+    --   : Term (.expression t1) →
+    --     Term (.expression t2) →
+    --     Term (.expression (t1 + t2))
 
-    | intersect
-      {n : ℕ}
-      {t1 t2 : RelType R n}
-      : Term (.expression t1) →
-        Term (.expression t2) →
-        Term (.expression (t1 & t2))
+    -- | intersect
+    --   {n : ℕ}
+    --   {t1 t2 : RelType R n}
+    --   : Term (.expression t1) →
+    --     Term (.expression t2) →
+    --     Term (.expression (t1 & t2))
 
-    | difference
-      {n : ℕ}
-      {t1 t2 : RelType R n}
-      : Term (.expression t1) →
-        Term (.expression t2) →
-        Term (.expression (t1 - t2))
+    -- | difference
+    --   {n : ℕ}
+    --   {t1 t2 : RelType R n}
+    --   : Term (.expression t1) →
+    --     Term (.expression t2) →
+    --     Term (.expression (t1 - t2))
 
-    | overwrite
-      {n : ℕ}
-      {t1 t2 : RelType R n}
-      : Term (.expression t1) →
-        Term (.expression t2) →
-        Term (.expression (t1 ++ t2))
+    -- | overwrite
+    --   {n : ℕ}
+    --   {t1 t2 : RelType R n}
+    --   : Term (.expression t1) →
+    --     Term (.expression t2) →
+    --     Term (.expression (t1 ++ t2))
 
-    | domain_restriction
-      {n : ℕ}
-      {t1 : RelType R 1}
-      {t2 : RelType R n}
-      : Term (.expression t1) →
-        Term (.expression t2) →
-        Term (.expression (t1 <: t2))
+    -- | domain_restriction
+    --   {n : ℕ}
+    --   {t1 : RelType R 1}
+    --   {t2 : RelType R n}
+    --   : Term (.expression t1) →
+    --     Term (.expression t2) →
+    --     Term (.expression (t1 <: t2))
 
-    | range_restriction
-      {n : ℕ}
-      {t1 : RelType R n}
-      {t2 : RelType R 1}
-      : Term (.expression t1) →
-        Term (.expression t2) →
-        Term (.expression (t1 :> t2))
+    -- | range_restriction
+    --   {n : ℕ}
+    --   {t1 : RelType R n}
+    --   {t2 : RelType R 1}
+    --   : Term (.expression t1) →
+    --     Term (.expression t2) →
+    --     Term (.expression (t1 :> t2))
 
-    | dotjoin
-      {n m : ℕ}
-      {t1 : RelType R (n+1)}
-      {t2 : RelType R (m+2)}
-      : Term (.expression t1) →
-        Term (.expression t2) →
-        Term (.expression (t1 ⋈ t2))
+    -- | dotjoin
+    --   {n m : ℕ}
+    --   {t1 : RelType R (n+1)}
+    --   {t2 : RelType R (m+2)}
+    --   : Term (.expression t1) →
+    --     Term (.expression t2) →
+    --     Term (.expression (t1 ⋈ t2))
 
-    /- unary expression operators -/
-    | transclos
-      {t : RelType R 2}
-      : Term (.expression t) →
-        Term (.expression (^ t))
+    -- /- unary expression operators -/
+    -- | transclos
+    --   {t : RelType R 2}
+    --   : Term (.expression t) →
+    --     Term (.expression (^ t))
 
-    | reflexive_closure
-      {t : RelType R 2}
-      : Term (.expression t) →
-        Term (.expression (* t))
+    -- | reflexive_closure
+    --   {t : RelType R 2}
+    --   : Term (.expression t) →
+    --     Term (.expression (* t))
 
-    | transposition
-      {t : RelType R 2}
-      : Term (.expression t) →
-        Term (.expression (~ t))
+    -- | transposition
+    --   {t : RelType R 2}
+    --   : Term (.expression t) →
+    --     Term (.expression (~ t))
 
-    /- expression if else -/
-    | if_then_else
-      {n : ℕ}
-      {t1 t2 : RelType R n}
-      : Term .formula →
-        Term (.expression t1) →
-        Term (.expression t2) →
-        Term (.expression (RelType.ifThenElse t1 t2))
+    -- /- expression if else -/
+    -- | if_then_else
+    --   {n : ℕ}
+    --   {t1 t2 : RelType R n}
+    --   : Term .formula →
+    --     Term (.expression t1) →
+    --     Term (.expression t2) →
+    --     Term (.expression (RelType.ifThenElse t1 t2))
 
-    /- function call from expression ? -/
-    --| call -- skip ?
+    -- /- function call from expression ? -/
+    -- --| call -- skip ?
 
-    /--bracket definition-/
-    | bracket : Term ty → Term ty
+    -- /--bracket definition-/
+    -- | bracket : Term ty → Term ty
 
-    /--predicate definition-/
-    | pred_def (name : String) : Term ty → Term ty
+    -- /--predicate definition-/
+    -- | pred_def (name : String) : Term ty → Term ty
 
-    /--function definition-/
-    | fun_def (name : String) : Term ty → Term ty
-    -- | marker : Marker → Term ty → Term ty
-    -- | name : String → Term ty → Term ty
+    -- /--function definition-/
+    -- | fun_def (name : String) : Term ty → Term ty
+    -- -- | marker : Marker → Term ty → Term ty
+    -- -- | name : String → Term ty → Term ty
 
-    /- algebra expression number -/
-    | number (z : ℤ) : Term .number -- may have to be from N
+    -- /- algebra expression number -/
+    -- | number (z : ℤ) : Term .number -- may have to be from N
 
-    /- algebra expression unary operation -/
-    | negation : Term .number → Term .number
+    -- /- algebra expression unary operation -/
+    -- | negation : Term .number → Term .number
 
-    /- algebra expression binary operation -/
-    | add
-      : Term .number →
-      Term .number →
-      Term .number
+    -- /- algebra expression binary operation -/
+    -- | add
+    --   : Term .number →
+    --   Term .number →
+    --   Term .number
 
-    | sub
-      : Term .number →
-      Term .number →
-      Term .number
+    -- | sub
+    --   : Term .number →
+    --   Term .number →
+    --   Term .number
 
-    | mul
-      : Term .number →
-        Term .number →
-        Term .number
+    -- | mul
+    --   : Term .number →
+    --     Term .number →
+    --     Term .number
 
-    | div
-      : Term .number →
-        Term .number →
-        Term .number
+    -- | div
+    --   : Term .number →
+    --     Term .number →
+    --     Term .number
 
-    | rem
-      : Term .number →
-        Term .number →
-        Term .number
+    -- | rem
+    --   : Term .number →
+    --     Term .number →
+    --     Term .number
 
-    /- algebra expression card operation (rel operation)-/
-    | card
-      {n : ℕ}
-      {t : RelType R n}
-      : Term (.expression t) →
-        Term .number
+    -- /- algebra expression card operation (rel operation)-/
+    -- | card
+    --   {n : ℕ}
+    --   {t : RelType R n}
+    --   : Term (.expression t) →
+    --     Term .number
 
-    /- formula unary rel bool operator-/
-    | no
-      {n : ℕ}
-      {t : RelType R n}
-      : Term (.expression t) →
-        Term .formula
+    -- /- formula unary rel bool operator-/
+    -- | no
+    --   {n : ℕ}
+    --   {t : RelType R n}
+    --   : Term (.expression t) →
+    --     Term .formula
 
-    | one
-      {n : ℕ}
-      {t : RelType R n}
-      : Term (.expression t) →
-        Term .formula
+    -- | one
+    --   {n : ℕ}
+    --   {t : RelType R n}
+    --   : Term (.expression t) →
+    --     Term .formula
 
-    | lone
-      {n : ℕ}
-      {t : RelType R n}
-      : Term (.expression t) →
-        Term .formula
+    -- | lone
+    --   {n : ℕ}
+    --   {t : RelType R n}
+    --   : Term (.expression t) →
+    --     Term .formula
 
-    | some
-      {n : ℕ}
-      {t : RelType R n}
-      : Term (.expression t) →
-        Term .formula
+    -- | some
+    --   {n : ℕ}
+    --   {t : RelType R n}
+    --   : Term (.expression t) →
+    --     Term .formula
 
-    /- formula unary logic operator -/
-    | not : Term .formula → Term .formula
+    -- /- formula unary logic operator -/
+    -- | not : Term .formula → Term .formula
 
-    /- formula binary logic operator -/
-    | or
-      : Term .formula →
-        Term .formula →
-        Term .formula
+    -- /- formula binary logic operator -/
+    -- | or
+    --   : Term .formula →
+    --     Term .formula →
+    --     Term .formula
 
-    | and
-      : Term .formula →
-        Term .formula →
-        Term .formula
+    -- | and
+    --   : Term .formula →
+    --     Term .formula →
+    --     Term .formula
 
-    | implication
-      : Term .formula →
-        Term .formula →
-        Term .formula
+    -- | implication
+    --   : Term .formula →
+    --     Term .formula →
+    --     Term .formula
 
-    | equivalent
-      : Term .formula →
-        Term .formula →
-        Term .formula
+    -- | equivalent
+    --   : Term .formula →
+    --     Term .formula →
+    --     Term .formula
 
-    /- formula if else-/
-    | f_if_then_else
-      : Term .formula →
-        Term .formula →
-        Term .formula →
-        Term .formula
+    -- /- formula if else-/
+    -- | f_if_then_else
+    --   : Term .formula →
+    --     Term .formula →
+    --     Term .formula →
+    --     Term .formula
 
-    /- formula algebraic comparison operator -/
-    | algebraic_leq
-      : Term .number →
-        Term .number →
-        Term .formula
+    -- /- formula algebraic comparison operator -/
+    -- | algebraic_leq
+    --   : Term .number →
+    --     Term .number →
+    --     Term .formula
 
-    | algebraic_geq
-      : Term .number →
-        Term .number →
-        Term .formula
+    -- | algebraic_geq
+    --   : Term .number →
+    --     Term .number →
+    --     Term .formula
 
-    | algebraic_eq
-      : Term .number →
-        Term .number →
-        Term .formula
+    -- | algebraic_eq
+    --   : Term .number →
+    --     Term .number →
+    --     Term .formula
 
-    | algebraic_lt
-      : Term .number →
-        Term .number →
-        Term .formula
+    -- | algebraic_lt
+    --   : Term .number →
+    --     Term .number →
+    --     Term .formula
 
-    | algebraic_gt
-      : Term .number →
-        Term .number →
-        Term .formula
+    -- | algebraic_gt
+    --   : Term .number →
+    --     Term .number →
+    --     Term .formula
 
     /- formula relation comparison operation -/
     | in
@@ -283,35 +283,35 @@ inductive TyTy : Type 1 where
         (expression2 : Term (.expression t2)) →
         Term .formula
 
-    | eq
-      {n : ℕ}
-      {t1 t2 : RelType R n}
-      : (expression1 : Term (.expression t1)) →
-        (expression2 : Term (.expression t2)) →
-        Term .formula
+    -- | eq
+    --   {n : ℕ}
+    --   {t1 t2 : RelType R n}
+    --   : (expression1 : Term (.expression t1)) →
+    --     (expression2 : Term (.expression t2)) →
+    --     Term .formula
 
-    | neq
-      {n : ℕ}
-      {t1 t2 : RelType R n}
-      : (expression1 : Term (.expression t1)) →
-        (expression2 : Term (.expression t2)) →
-        Term .formula
+    -- | neq
+    --   {n : ℕ}
+    --   {t1 t2 : RelType R n}
+    --   : (expression1 : Term (.expression t1)) →
+    --     (expression2 : Term (.expression t2)) →
+    --     Term .formula
 
-    /- function abstraction -/
-    | lam (t : RelType R n)
-      : (Rel t → Term ran) →
-        Term (.function t ran)
+    -- /- function abstraction -/
+    -- | lam (t : RelType R n)
+    --   : (Rel t → Term ran) →
+    --     Term (.function t ran)
 
-    /- function application / application of argument to call ? -/
-    | app
-      : Term (.function t ran) →
-        Term (.expression t) →
-        Term ran
+    -- /- function application / application of argument to call ? -/
+    -- | app
+    --   : Term (.function t ran) →
+    --     Term (.expression t) →
+    --     Term ran
 
-    | q_group
-      : Shared.quant →
-        Term .formula →
-        Term .formula
+    -- | q_group
+    --   : Shared.quant →
+    --     Term .formula →
+    --     Term .formula
 
     | pred_1 {n : ℕ} {t : RelType R n}
       : (Rel t → Term .formula) →
@@ -331,313 +331,354 @@ inductive TyTy : Type 1 where
         (parameter : Term (.expression t)) →
         Term ran
 
-  def Term.eval
-    {R : Type}
-    [TupleSet R]
-    {tt : TyTy}
-    {ty : @Ty R _ tt}
-    (t : @Term R _ _ ty)
-    : ty.eval :=
-      match t with
 
-      | .global_rel_var r _ => r
-      | .local_rel_var r => r
-
-      /- binary expression operators -/
-      | .intersect r1 r2 => (r1.eval) & (r2.eval)
-      | .union r1 r2 => HAdd.hAdd (r1.eval) (r2.eval)
-      | .difference r1 r2 => (r1.eval) - (r2.eval)
-      | .overwrite r1 r2 => (r1.eval) ++ (r2.eval)
-      | .domain_restriction r1 r2 => (r1.eval) <: (r2.eval)
-      | .range_restriction r1 r2 => (r1.eval) :> (r2.eval)
-      | .dotjoin r1 r2 => (r1.eval) ⋈ (r2.eval)
-
-      /- unary expression operators -/
-      | .transclos r => ^ (r.eval)
-      | .reflexive_closure  r => * (r.eval)
-      | .transposition r => ~ (r.eval)
-
-      /- expression if else -/
-      | .if_then_else f r1 r2 => HIfThenElse.hIfThenElse (f.eval) (r1.eval) (r2.eval)
-
-      | .bracket t => t.eval
-      | .pred_def _ t => t.eval
-      | .fun_def _ t => t.eval
-      -- | .marker _ t => t.eval
-      -- | .name _ t => t.eval
-
-      | @Term.lam R _ _ _ t f => λ (x : Rel t) => (f x).eval
-      | .app f r => f.eval r.eval
-
-      | .q_group m p => p.eval
-
-      | .pred_1 f => λ x => (f x).eval
-      | .pred_n f => λ x => (f x).eval
-
-      | .bind_1 m f x => ∀ x, f.eval x
-      | @Term.bind_n R _ _ t ran m f x => ( ∀ x, (Term.eval f) x : (Ty.eval ty) )
-
-      | .number z => z
-
-      /- algebra expression unary operation -/
-      | .negation z => - (z.eval)
-
-      /- algebra expression binary operation -/
-      | .add z1 z2 => (z1.eval) + (z2.eval)
-      | .sub z1 z2 => (z1.eval) - (z2.eval)
-      | .div z1 z2 => (z1.eval) / (z2.eval)
-      | .mul z1 z2 => (z1.eval) * (z2.eval)
-      | .rem z1 z2 => (z1.eval) % (z2.eval)
-
-      /- algebra expression card operation (rel operation)-/
-      | .card r => Card.card (r.eval)
-
-      /- formula unary rel bool operator-/
-      | .no r => SetMultPredicates.no (r.eval)
-      | .one r => SetMultPredicates.one (r.eval)
-      | .lone r => SetMultPredicates.lone (r.eval)
-      | .some r => SetMultPredicates.some (r.eval)
-
-      /- formula unary logic operator -/
-      | .not f => ¬ (f.eval)
-
-      /- formula binary logic operator -/
-      | .or f1 f2 => (f1.eval) ∨ (f2.eval)
-      | .and f1 f2 => (f1.eval) ∧ (f2.eval)
-      | .implication f1 f2 => (f1.eval) → (f2.eval)
-      | .equivalent f1 f2 => (f1.eval) = (f2.eval)
-
-      /- formula if else -/
-      | .f_if_then_else f1 f2 f3 =>
-        ((f1.eval) -> (f2.eval)) ∧ (¬ (f1.eval) → (f2.eval))
-
-      /- formula algebraic comparison operator -/
-      | .algebraic_leq z1 z2 => (z1.eval) <= (z2.eval)
-      | .algebraic_geq z1 z2 => (z1.eval) >= (z2.eval)
-      | .algebraic_lt z1 z2 => (z1.eval) < (z2.eval)
-      | .algebraic_gt z1 z2 => (z1.eval) > (z2.eval)
-      | .algebraic_eq z1 z2 => (z1.eval) = (z2.eval)
-
-      /- formula relation comparison operation -/
-      | .in r1 r2 => (r1.eval) ⊂ (r2.eval)
-      | .eq r1 r2 => (r1.eval) ≡ (r2.eval)
-      | .neq r1 r2 => (r1.eval) ≢  (r2.eval)
-
-      -- | q_group {t : RelType R n} {ran : Ty (.isPred t)}
-      --     : Shared.quant →
-      --       Term ran →
-      --       Term .formula
-
-  instance {R : Type} [TupleSet R] {ty : @Ty R _} (t : @Term R _ ty):
-    CoeDep (@Term R _ ty) t ty.eval where
-      coe := t.eval
-
-  instance {R : Type} [TupleSet R] {n : ℕ} (t : @Term R _ (Ty.type n)):
-    CoeDep _ t Type where
-      coe := Rel t.eval
-
-end ThoR.Semantics
-
-/-
-all disj x, y, z : r | ...
-
-->
-all disj x : r | all y : r | all z : r | ...
-
-
--/
-open ThoR.Semantics
-open ThoR
-
--- automatic coercion from t : RelType to Rel t : Type
-instance {R : Type} [ThoR.TupleSet R] {n : ℕ} (t : RelType R n):
-  CoeDep (RelType R n ) t Type where
-    coe := ThoR.Rel t
-
-variable (R : Type) [TupleSet R]
-#check ThoR.Rel (RelType.mk.sig R Shared.mult.set)
-
-class vars (R : Type) [TupleSet R] where
-  UNIV : ((RelType.mk.sig R Shared.mult.set) : Type)
-  Time : Rel (RelType.mk.sig R Shared.mult.set)
-
-variable (ThoR_TupleSet : Type) [TupleSet ThoR_TupleSet] [vars ThoR_TupleSet]
-
-@[default_instance]
-instance : ThoR.TupleSet ThoR_TupleSet := by sorry
-
-@[default_instance]
-instance : vars ThoR_TupleSet := by sorry
-
-/-
-pred_in1 [x : set univ] {
- x in x
-}
--/
-def pred_in1 :=
-  Term.pred_def "p1" (
-  -- @Term.marker ThoR_TupleSet _ [] _ Marker.alloy_predicate (
-  --   @Term.name ThoR_TupleSet _ _ _ "pred_in1" (
-      Term.lam _ (
-        λ (r : (Rel (RelType.mk.sig ThoR_TupleSet Shared.mult.set))) =>
-          Term.in
-            (expression1 := Term.local_rel_var r)
-            (expression2 := Term.local_rel_var r)
-      )
-      )
-
-/-
-pred_in2 [x : set univ] {
-  x in m/UNIV
-}
--/
-def pred_in2 :=
-  Term.pred_def "p2" (
-    Term.lam _ (
-      λ (x : (Rel (RelType.mk.sig ThoR_TupleSet Shared.mult.set))) =>
+variable {R : Type} [TupleSet R] (t : RelType R n)
+#check Term.pred_1 (λ (r : Rel t) => Term.in
+              (expression1 := Term.local_rel_var r)
+              (expression2 := Term.local_rel_var r) )
+#check Term.pred_n (
+    λ (q : Rel t) => Term.pred_1 (
+      λ (r : Rel t) =>
         Term.in
-          (expression1 := Term.local_rel_var x)
-          (expression2 := Term.global_rel_var (@vars.UNIV ThoR_TupleSet _ _) "m/UNIV")
-    )
-  )
+          (expression1 := Term.local_rel_var q)
+          (expression2 := Term.local_rel_var r)
+      )
+)
 
-#check (pred_in1 ThoR_TupleSet)
-#check (
-  Term.app
-    (pred_in1 ThoR_TupleSet)
-    (Term.global_rel_var (@vars.UNIV ThoR_TupleSet _ _) "UNIV")
-  ).eval
+def p1 := Term.pred_n (
+    λ (q : Rel t) => Term.pred_1 (
+      λ (r : Rel t) =>
+        Term.in
+          (expression1 := Term.local_rel_var q)
+          (expression2 := Term.local_rel_var r)
+      )
+)
 
--- pred_in1[univ]
-example : (Term.app (pred_in1 ThoR_TupleSet) (Term.global_rel_var (@vars.UNIV ThoR_TupleSet _ _) "UNIV")).eval := by
-  dsimp [Term.eval]
-  apply Set.subset_refl
 
--- pred_in2[univ]
-example : (
-  Term.app
-    (pred_in2 ThoR_TupleSet)
-    (Term.global_rel_var (@vars.UNIV ThoR_TupleSet _ _) "m/UNIV")
-  ).eval := by
-  dsimp [Term.eval]
-  apply Set.subset_refl
-
-/-
-pred_in3 [x : set univ, y : set univ] {
-  x in y
-}
--/
-def pred_in3 :=
-  Term.pred_def "p3" (
-    Term.lam _ (
-      λ (x : (Rel (RelType.mk.sig ThoR_TupleSet Shared.mult.set))) =>
-        Term.lam _ (
-          λ (y : (Rel (RelType.mk.sig ThoR_TupleSet Shared.mult.set))) =>
-            Term.in
-              (expression1 := Term.local_rel_var x)
-              (expression2 := Term.local_rel_var y)
-        )
-    )
-  )
-
--- pred_in3[univ,univ]
-example : (
-  Term.app
-    (Term.app
-      (@pred_in3 ThoR_TupleSet _)
-      (Term.global_rel_var (@vars.UNIV ThoR_TupleSet _ _) "m/UNIV")
-    )
-    (Term.global_rel_var (@vars.UNIV ThoR_TupleSet _ _) "m/UNIV")
-  ).eval := by
-    dsimp [Term.eval]
-    apply Set.subset_refl
-
-/-
-fun1 [x : set univ, y : set univ] : univ {
-  x & y
-}
--/
-def fun1 :=
-  Term.fun_def "f1" (
-    Term.lam _ (
-      λ (x : (Rel (RelType.mk.sig ThoR_TupleSet Shared.mult.set))) =>
-        Term.lam _ (
-          λ (y : (Rel (RelType.mk.sig ThoR_TupleSet Shared.mult.set))) =>
-            Term.intersect
-              (Term.local_rel_var x)
-              (Term.local_rel_var y)
-        )
-    )
-  )
-
-/-
-fun2 [r : set univ] : univ {
-  fun1 r
-}
--/
-def fun2 :=
-  Term.fun_def "f2" (
-    Term.lam _ (
-      λ (r : (Rel (RelType.mk.sig ThoR_TupleSet Shared.mult.set))) =>
-        ( Term.app
-          (Term.app
-            (fun1 ThoR_TupleSet) (Term.local_rel_var r)
-          )
-          (Term.local_rel_var r))
-    )
-  )
-
-/-
-fun1 [r : set univ] : univ {
-  r + r
-}
--/
-def fun_union1 :=
-    Term.lam _ (
-      λ (r : (Rel (RelType.mk.sig ThoR_TupleSet Shared.mult.set))) =>
-        Term.union
-          (Term.local_rel_var r)
-          (Term.local_rel_var r)
-    )
-
-#check (Term.app (fun_union1 ThoR_TupleSet) (Term.global_rel_var (@vars.UNIV ThoR_TupleSet _ _) "UNIV")).eval
--- pred_in1[univ]
-example : (Term.app (fun_union1 ThoR_TupleSet) (Term.global_rel_var (@vars.UNIV ThoR_TupleSet _ _) "UNIV")).eval =  (@vars.UNIV ThoR_TupleSet _ _) + (@vars.UNIV ThoR_TupleSet _ _) := by
-  dsimp [Term.eval]
-
-/-
-fun1 [r : set univ] : univ {
-  fun_union1 r + fun_union1 r
-}
--/
-def fun_union_union :=
-    Term.lam _ (
-      λ (r : (Rel (RelType.mk.sig ThoR_TupleSet Shared.mult.set))) =>
-        Term.union
-          (Term.app (fun_union1 ThoR_TupleSet) (Term.local_rel_var r))
-          (Term.app (fun_union1 ThoR_TupleSet) (Term.local_rel_var r))
-    )
-#check (Term.app (fun_union_union ThoR_TupleSet) (Term.global_rel_var (@vars.UNIV ThoR_TupleSet _ _) "UNIV")).eval
-
+#check (p1 t)
 
 -- set_option diagnostics true
-example : (Term.app (fun_union_union ThoR_TupleSet) (Term.global_rel_var (@vars.UNIV ThoR_TupleSet _ _) "UNIV")).eval = ((@vars.UNIV ThoR_TupleSet _ _) + (@vars.UNIV ThoR_TupleSet _ _)) + ((@vars.UNIV ThoR_TupleSet _ _) + (@vars.UNIV ThoR_TupleSet _ _)) := by
---  unfold Term.eval
-  dsimp [Term.eval]
+-- set_option diagnostics.threshold 0
 
-#check Term.union (Term.global_rel_var (@vars.UNIV ThoR_TupleSet _ _) "UNIV") (Term.global_rel_var (@vars.UNIV ThoR_TupleSet _ _) "UNIV")
+example : p1 t = Term.pred_n (
+    λ (q : Rel t) => Term.pred_1 (
+      λ (r : Rel t) =>
+        Term.in
+          (expression1 := Term.local_rel_var q)
+          (expression2 := Term.local_rel_var r)
+      )
+) := by
+  cases
 
-#check Term.union (Term.union (Term.global_rel_var (@vars.UNIV ThoR_TupleSet _ _) "UNIV") (Term.global_rel_var (@vars.UNIV ThoR_TupleSet _ _) "UNIV")) (Term.union (Term.global_rel_var (@vars.UNIV ThoR_TupleSet _ _) "UNIV") (Term.global_rel_var (@vars.UNIV ThoR_TupleSet _ _) "UNIV"))
 
-example : (Term.app (fun_union_union ThoR_TupleSet) (Term.global_rel_var (@vars.UNIV ThoR_TupleSet _ _) "UNIV")).eval = (Term.union (Term.union (Term.global_rel_var (@vars.UNIV ThoR_TupleSet _ _) "UNIV") (Term.global_rel_var (@vars.UNIV ThoR_TupleSet _ _) "UNIV")) (Term.union (Term.global_rel_var (@vars.UNIV ThoR_TupleSet _ _) "UNIV") (Term.global_rel_var (@vars.UNIV ThoR_TupleSet _ _) "UNIV"))).eval := by
-  dsimp [Term.eval]
 
-example : (Term.app (fun_union_union ThoR_TupleSet) (Term.global_rel_var (@vars.UNIV ThoR_TupleSet _ _) "UNIV")).eval ≡ ((@vars.UNIV ThoR_TupleSet _ _) + (@vars.UNIV ThoR_TupleSet _ _)) + ((@vars.UNIV ThoR_TupleSet _ _) + (@vars.UNIV ThoR_TupleSet _ _)) := by
-  dsimp [Term.eval]
-  dsimp [HEqual.hEqual]
+--   def Term.eval
+--     {R : Type}
+--     [TupleSet R]
+--     {tt : TyTy}
+--     {ty : @Ty R _ tt}
+--     (t : @Term R _ _ ty)
+--     : ty.eval :=
+--       match t with
 
-example : (Term.app (fun_union_union ThoR_TupleSet) (Term.global_rel_var (@vars.UNIV ThoR_TupleSet _ _) "UNIV")).eval ≡ (@vars.UNIV ThoR_TupleSet _ _) + (@vars.UNIV ThoR_TupleSet _ _) + (@vars.UNIV ThoR_TupleSet _ _) + (@vars.UNIV ThoR_TupleSet _ _) := by
-  dsimp [Term.eval]
-  -- TODO apply rewrite-lemma for associativity of +
-  dsimp [HEqual.hEqual]
-  sorry
+--       | .global_rel_var r _ => r
+--       | .local_rel_var r => r
+
+--       /- binary expression operators -/
+--       | .intersect r1 r2 => (r1.eval) & (r2.eval)
+--       | .union r1 r2 => HAdd.hAdd (r1.eval) (r2.eval)
+--       | .difference r1 r2 => (r1.eval) - (r2.eval)
+--       | .overwrite r1 r2 => (r1.eval) ++ (r2.eval)
+--       | .domain_restriction r1 r2 => (r1.eval) <: (r2.eval)
+--       | .range_restriction r1 r2 => (r1.eval) :> (r2.eval)
+--       | .dotjoin r1 r2 => (r1.eval) ⋈ (r2.eval)
+
+--       /- unary expression operators -/
+--       | .transclos r => ^ (r.eval)
+--       | .reflexive_closure  r => * (r.eval)
+--       | .transposition r => ~ (r.eval)
+
+--       /- expression if else -/
+--       | .if_then_else f r1 r2 => HIfThenElse.hIfThenElse (f.eval) (r1.eval) (r2.eval)
+
+--       | .bracket t => t.eval
+--       | .pred_def _ t => t.eval
+--       | .fun_def _ t => t.eval
+--       -- | .marker _ t => t.eval
+--       -- | .name _ t => t.eval
+
+--       | @Term.lam R _ _ _ t f => λ (x : Rel t) => (f x).eval
+--       | .app f r => f.eval r.eval
+
+--       | .q_group m p => p.eval
+
+--       | .pred_1 f => λ x => (f x).eval
+--       | @Term.pred_n R _ n t ran f => ( λ x => (f x).eval : Rel t → ran.eval )
+
+--       | .bind_1 m f x => ∀ x, f.eval x
+--       | @Term.bind_n R _ _ t ran m f x => ( ∀ x, ((Term.eval f) x ) : ty.eval )
+
+--       | .number z => z
+
+--       /- algebra expression unary operation -/
+--       | .negation z => - (z.eval)
+
+--       /- algebra expression binary operation -/
+--       | .add z1 z2 => (z1.eval) + (z2.eval)
+--       | .sub z1 z2 => (z1.eval) - (z2.eval)
+--       | .div z1 z2 => (z1.eval) / (z2.eval)
+--       | .mul z1 z2 => (z1.eval) * (z2.eval)
+--       | .rem z1 z2 => (z1.eval) % (z2.eval)
+
+--       /- algebra expression card operation (rel operation)-/
+--       | .card r => Card.card (r.eval)
+
+--       /- formula unary rel bool operator-/
+--       | .no r => SetMultPredicates.no (r.eval)
+--       | .one r => SetMultPredicates.one (r.eval)
+--       | .lone r => SetMultPredicates.lone (r.eval)
+--       | .some r => SetMultPredicates.some (r.eval)
+
+--       /- formula unary logic operator -/
+--       | .not f => ¬ (f.eval)
+
+--       /- formula binary logic operator -/
+--       | .or f1 f2 => (f1.eval) ∨ (f2.eval)
+--       | .and f1 f2 => (f1.eval) ∧ (f2.eval)
+--       | .implication f1 f2 => (f1.eval) → (f2.eval)
+--       | .equivalent f1 f2 => (f1.eval) = (f2.eval)
+
+--       /- formula if else -/
+--       | .f_if_then_else f1 f2 f3 =>
+--         ((f1.eval) -> (f2.eval)) ∧ (¬ (f1.eval) → (f2.eval))
+
+--       /- formula algebraic comparison operator -/
+--       | .algebraic_leq z1 z2 => (z1.eval) <= (z2.eval)
+--       | .algebraic_geq z1 z2 => (z1.eval) >= (z2.eval)
+--       | .algebraic_lt z1 z2 => (z1.eval) < (z2.eval)
+--       | .algebraic_gt z1 z2 => (z1.eval) > (z2.eval)
+--       | .algebraic_eq z1 z2 => (z1.eval) = (z2.eval)
+
+--       /- formula relation comparison operation -/
+--       | .in r1 r2 => (r1.eval) ⊂ (r2.eval)
+--       | .eq r1 r2 => (r1.eval) ≡ (r2.eval)
+--       | .neq r1 r2 => (r1.eval) ≢  (r2.eval)
+
+--       -- | q_group {t : RelType R n} {ran : Ty (.isPred t)}
+--       --     : Shared.quant →
+--       --       Term ran →
+--       --       Term .formula
+
+--   instance {R : Type} [TupleSet R] {ty : @Ty R _} (t : @Term R _ ty):
+--     CoeDep (@Term R _ ty) t ty.eval where
+--       coe := t.eval
+
+--   instance {R : Type} [TupleSet R] {n : ℕ} (t : @Term R _ (Ty.type n)):
+--     CoeDep _ t Type where
+--       coe := Rel t.eval
+
+-- end ThoR.Semantics
+
+-- /-
+-- all disj x, y, z : r | ...
+
+-- ->
+-- all disj x : r | all y : r | all z : r | ...
+
+
+-- -/
+-- open ThoR.Semantics
+-- open ThoR
+
+-- -- automatic coercion from t : RelType to Rel t : Type
+-- instance {R : Type} [ThoR.TupleSet R] {n : ℕ} (t : RelType R n):
+--   CoeDep (RelType R n ) t Type where
+--     coe := ThoR.Rel t
+
+-- variable (R : Type) [TupleSet R]
+-- #check ThoR.Rel (RelType.mk.sig R Shared.mult.set)
+
+-- class vars (R : Type) [TupleSet R] where
+--   UNIV : ((RelType.mk.sig R Shared.mult.set) : Type)
+--   Time : Rel (RelType.mk.sig R Shared.mult.set)
+
+-- variable (ThoR_TupleSet : Type) [TupleSet ThoR_TupleSet] [vars ThoR_TupleSet]
+
+-- @[default_instance]
+-- instance : ThoR.TupleSet ThoR_TupleSet := by sorry
+
+-- @[default_instance]
+-- instance : vars ThoR_TupleSet := by sorry
+
+-- /-
+-- pred_in1 [x : set univ] {
+--  x in x
+-- }
+-- -/
+-- def pred_in1 :=
+--   Term.pred_def "p1" (
+--   -- @Term.marker ThoR_TupleSet _ [] _ Marker.alloy_predicate (
+--   --   @Term.name ThoR_TupleSet _ _ _ "pred_in1" (
+--       Term.lam _ (
+--         λ (r : (Rel (RelType.mk.sig ThoR_TupleSet Shared.mult.set))) =>
+--           Term.in
+--             (expression1 := Term.local_rel_var r)
+--             (expression2 := Term.local_rel_var r)
+--       )
+--       )
+
+-- /-
+-- pred_in2 [x : set univ] {
+--   x in m/UNIV
+-- }
+-- -/
+-- def pred_in2 :=
+--   Term.pred_def "p2" (
+--     Term.lam _ (
+--       λ (x : (Rel (RelType.mk.sig ThoR_TupleSet Shared.mult.set))) =>
+--         Term.in
+--           (expression1 := Term.local_rel_var x)
+--           (expression2 := Term.global_rel_var (@vars.UNIV ThoR_TupleSet _ _) "m/UNIV")
+--     )
+--   )
+
+-- #check (pred_in1 ThoR_TupleSet)
+-- #check (
+--   Term.app
+--     (pred_in1 ThoR_TupleSet)
+--     (Term.global_rel_var (@vars.UNIV ThoR_TupleSet _ _) "UNIV")
+--   ).eval
+
+-- -- pred_in1[univ]
+-- example : (Term.app (pred_in1 ThoR_TupleSet) (Term.global_rel_var (@vars.UNIV ThoR_TupleSet _ _) "UNIV")).eval := by
+--   dsimp [Term.eval]
+--   apply Set.subset_refl
+
+-- -- pred_in2[univ]
+-- example : (
+--   Term.app
+--     (pred_in2 ThoR_TupleSet)
+--     (Term.global_rel_var (@vars.UNIV ThoR_TupleSet _ _) "m/UNIV")
+--   ).eval := by
+--   dsimp [Term.eval]
+--   apply Set.subset_refl
+
+-- /-
+-- pred_in3 [x : set univ, y : set univ] {
+--   x in y
+-- }
+-- -/
+-- def pred_in3 :=
+--   Term.pred_def "p3" (
+--     Term.lam _ (
+--       λ (x : (Rel (RelType.mk.sig ThoR_TupleSet Shared.mult.set))) =>
+--         Term.lam _ (
+--           λ (y : (Rel (RelType.mk.sig ThoR_TupleSet Shared.mult.set))) =>
+--             Term.in
+--               (expression1 := Term.local_rel_var x)
+--               (expression2 := Term.local_rel_var y)
+--         )
+--     )
+--   )
+
+-- -- pred_in3[univ,univ]
+-- example : (
+--   Term.app
+--     (Term.app
+--       (@pred_in3 ThoR_TupleSet _)
+--       (Term.global_rel_var (@vars.UNIV ThoR_TupleSet _ _) "m/UNIV")
+--     )
+--     (Term.global_rel_var (@vars.UNIV ThoR_TupleSet _ _) "m/UNIV")
+--   ).eval := by
+--     dsimp [Term.eval]
+--     apply Set.subset_refl
+
+-- /-
+-- fun1 [x : set univ, y : set univ] : univ {
+--   x & y
+-- }
+-- -/
+-- def fun1 :=
+--   Term.fun_def "f1" (
+--     Term.lam _ (
+--       λ (x : (Rel (RelType.mk.sig ThoR_TupleSet Shared.mult.set))) =>
+--         Term.lam _ (
+--           λ (y : (Rel (RelType.mk.sig ThoR_TupleSet Shared.mult.set))) =>
+--             Term.intersect
+--               (Term.local_rel_var x)
+--               (Term.local_rel_var y)
+--         )
+--     )
+--   )
+
+-- /-
+-- fun2 [r : set univ] : univ {
+--   fun1 r
+-- }
+-- -/
+-- def fun2 :=
+--   Term.fun_def "f2" (
+--     Term.lam _ (
+--       λ (r : (Rel (RelType.mk.sig ThoR_TupleSet Shared.mult.set))) =>
+--         ( Term.app
+--           (Term.app
+--             (fun1 ThoR_TupleSet) (Term.local_rel_var r)
+--           )
+--           (Term.local_rel_var r))
+--     )
+--   )
+
+-- /-
+-- fun1 [r : set univ] : univ {
+--   r + r
+-- }
+-- -/
+-- def fun_union1 :=
+--     Term.lam _ (
+--       λ (r : (Rel (RelType.mk.sig ThoR_TupleSet Shared.mult.set))) =>
+--         Term.union
+--           (Term.local_rel_var r)
+--           (Term.local_rel_var r)
+--     )
+
+-- #check (Term.app (fun_union1 ThoR_TupleSet) (Term.global_rel_var (@vars.UNIV ThoR_TupleSet _ _) "UNIV")).eval
+-- -- pred_in1[univ]
+-- example : (Term.app (fun_union1 ThoR_TupleSet) (Term.global_rel_var (@vars.UNIV ThoR_TupleSet _ _) "UNIV")).eval =  (@vars.UNIV ThoR_TupleSet _ _) + (@vars.UNIV ThoR_TupleSet _ _) := by
+--   dsimp [Term.eval]
+
+-- /-
+-- fun1 [r : set univ] : univ {
+--   fun_union1 r + fun_union1 r
+-- }
+-- -/
+-- def fun_union_union :=
+--     Term.lam _ (
+--       λ (r : (Rel (RelType.mk.sig ThoR_TupleSet Shared.mult.set))) =>
+--         Term.union
+--           (Term.app (fun_union1 ThoR_TupleSet) (Term.local_rel_var r))
+--           (Term.app (fun_union1 ThoR_TupleSet) (Term.local_rel_var r))
+--     )
+-- #check (Term.app (fun_union_union ThoR_TupleSet) (Term.global_rel_var (@vars.UNIV ThoR_TupleSet _ _) "UNIV")).eval
+
+
+-- -- set_option diagnostics true
+-- example : (Term.app (fun_union_union ThoR_TupleSet) (Term.global_rel_var (@vars.UNIV ThoR_TupleSet _ _) "UNIV")).eval = ((@vars.UNIV ThoR_TupleSet _ _) + (@vars.UNIV ThoR_TupleSet _ _)) + ((@vars.UNIV ThoR_TupleSet _ _) + (@vars.UNIV ThoR_TupleSet _ _)) := by
+-- --  unfold Term.eval
+--   dsimp [Term.eval]
+
+-- #check Term.union (Term.global_rel_var (@vars.UNIV ThoR_TupleSet _ _) "UNIV") (Term.global_rel_var (@vars.UNIV ThoR_TupleSet _ _) "UNIV")
+
+-- #check Term.union (Term.union (Term.global_rel_var (@vars.UNIV ThoR_TupleSet _ _) "UNIV") (Term.global_rel_var (@vars.UNIV ThoR_TupleSet _ _) "UNIV")) (Term.union (Term.global_rel_var (@vars.UNIV ThoR_TupleSet _ _) "UNIV") (Term.global_rel_var (@vars.UNIV ThoR_TupleSet _ _) "UNIV"))
+
+-- example : (Term.app (fun_union_union ThoR_TupleSet) (Term.global_rel_var (@vars.UNIV ThoR_TupleSet _ _) "UNIV")).eval = (Term.union (Term.union (Term.global_rel_var (@vars.UNIV ThoR_TupleSet _ _) "UNIV") (Term.global_rel_var (@vars.UNIV ThoR_TupleSet _ _) "UNIV")) (Term.union (Term.global_rel_var (@vars.UNIV ThoR_TupleSet _ _) "UNIV") (Term.global_rel_var (@vars.UNIV ThoR_TupleSet _ _) "UNIV"))).eval := by
+--   dsimp [Term.eval]
+
+-- example : (Term.app (fun_union_union ThoR_TupleSet) (Term.global_rel_var (@vars.UNIV ThoR_TupleSet _ _) "UNIV")).eval ≡ ((@vars.UNIV ThoR_TupleSet _ _) + (@vars.UNIV ThoR_TupleSet _ _)) + ((@vars.UNIV ThoR_TupleSet _ _) + (@vars.UNIV ThoR_TupleSet _ _)) := by
+--   dsimp [Term.eval]
+--   dsimp [HEqual.hEqual]
+
+-- example : (Term.app (fun_union_union ThoR_TupleSet) (Term.global_rel_var (@vars.UNIV ThoR_TupleSet _ _) "UNIV")).eval ≡ (@vars.UNIV ThoR_TupleSet _ _) + (@vars.UNIV ThoR_TupleSet _ _) + (@vars.UNIV ThoR_TupleSet _ _) + (@vars.UNIV ThoR_TupleSet _ _) := by
+--   dsimp [Term.eval]
+--   -- TODO apply rewrite-lemma for associativity of +
+--   dsimp [HEqual.hEqual]
+--   sorry
